---
title: "[Func-Num] Sequence and Series"

categories:
  - Func-Num
tags:
  - [Sequence, Series]

toc: true
toc_sticky: true

date: 2023-04-16
last_modified_at: 2023-04-16
---

<!-- {% capture notice-2 %}

üìã This is the tech-news archives to help me keep track of what I am interested in!

- Reference tech news link: <https://thenextweb.com/news/blockchain-development-tech-career>
  {% endcapture %}

<div class="notice--danger">{{ notice-2 | markdownify }}</div> -->

üìã This is my note-taking from what I learned in the class "Math175-002 Functions & Number Systems"
{: .notice--danger}

<br>

# Linear Growth and Arithmetic Sequence

Suppose that you earn $30 each day. If you start out with $100 in your savings, and you add the $30 to your savings every evening, how much will you have saved after 11 days?

| Days | Amount($) | Analysis     |
| :--- | :-------- | :----------- |
| 0    | 100       | 100 + 1 x 30 |
| 1    | 130       | 100 + 2 x 30 |
| 2    | 160       | 100 + 3 x 30 |

There is a pattern in the growth of the amount. At the end of the 11th day, you will have:

100 + 11 x 30 = $430 saved.

This additive growth is called linear growth.

<br>

## 1. Arithmetic Sequence

In an arithmetic sequence, the number obtained by subtracting any two consecutive terms is a constant. This constant "d" is called the "common difference" where "d = t<sub>n+1</sub> - t<sub>n</sub>"; subscript indicates order of term in the sequence.

Ex) 4, 9, 14, 19 ... &rarr; d = 9 - 4 = 5

## Example: 1. Arithmetic Sequence

1. State the common difference of arithmetic sequence: a) 25, 21, 17, ...

> d = t<sub>n+1</sub> - t<sub>n</sub>

| Answer           |
| :--------------- |
| d = 21 -‚ÄÑ25 = -4 |

<br>

## 1 - a. The general term of the arithmetic sequence

a, a + d, a + 2d, a + 3d, ‚Ä¶ is "t<sub>n</sub> = a + (n - 1)d," n is order of term in the sequence.

Ex) Determine the 30th term of the arithmetic sequence 4, 7, 10, ...

> d = t<sub>n+1</sub> - t<sub>n</sub>
>
> t<sub>n</sub> = a + (n - 1)d

| Solution                                          |
| :------------------------------------------------ |
| d = 7 -‚ÄÑ4 = 3                                     |
| t<sub>30</sub> = 4 + (30 - 1)(3) = 4 + 29(3) = 91 |

## Example: 1 - a. The general term of the arithmetic sequence

Determine the indicated term of the arithmetic sequence: 23, 34, 45, ... 10th term.

| Solution                                              |
| :---------------------------------------------------- |
| d = 34 -‚ÄÑ23 = 11                                      |
| t<sub>10</sub> = 23 + (10 - 1)(11) = 23 + 9(11) = 122 |

<br>

## 1 - b. The Sum of an Arithmetic Series

For the general arithmetic series "a + (a + d) + (a + 2d) + ... + t<sub>n</sub>," the sum of the first n terms is:

- S<sub>n</sub> =
  $$ {n} \over {2} $$
  (a + t<sub>n</sub>) &rarr; Use if last term is given!
- S<sub>n</sub> =
  $$ {n} \over {2} $$
  [2a + (n - 1)d]

Ex) 1. Determine the sum of the first 30th terms of the arithmetic series: 5 + 5.3 + 5.6 + ...

> S<sub>n</sub> =
> $$ {n} \over {2} $$
> [2a + (n - 1)d]

a = 5, d = 0.3, n = 30

| Solution                                             |
| :--------------------------------------------------- |
| S<sub>30</sub> = (30/2) [2(5) + (30 ‚Äì 1)0.3] = 280.5 |

Ex) 2. Determine the sum of the arithmetic series "‚Äì4, ‚Äì10, ‚Äì16, ..., -94"

> t<sub>n</sub> = a + (n - 1)d

nth term = -94, d = -6. So, what is n = ?

| Solution                     |
| :--------------------------- |
| t<sub>n</sub> = a + (n - 1)d |
| -94 = -4 + (n - 1)(-6)       |
| - 94 + 4 = -6n + 6           |
| - 90 - 6 = -6n               |
| -96 = -6n                    |
| -96/-6 = n                   |
| n = 16                       |

> S<sub>n</sub> =
> $$ {n} \over {2} $$
> (a + t<sub>n</sub>) &rarr; Use if last term is given!

We know that there are 16th terms in the series and that the 16th term is ‚Äì 94.

| Solution                              |
| :------------------------------------ |
| S<sub>16</sub> = 16/2(-4 - 94) = -784 |

## Example: 1 - b. The Sum of an Arithmetic Series

1. Determine the sum of the first 8 terms of the arithmetic sequence: 1.24 + 1.28 + 1.32 + ...

> S<sub>n</sub> =
> $$ {n} \over {2} $$
> [2a + (n - 1)d]

| Solution                                             |
| :--------------------------------------------------- |
| a = 1.24, d = 0.04, n = 8                            |
| S<sub>8</sub> = (8/2)[2(1.24) + (8-1)(0.04)] = 11.04 |

2. For the arithmetic sequence, a last term in the sequence is given, what is its order (subscript n)? what is the sum of the of the sequence? Sequence: 2, 7, 12, 17, ..., 187.

> t<sub>n</sub> = a + (n - 1)d

| Solution                          |
| :-------------------------------- |
| nth term = 187, d = 5, what is n? |
| 187 = 2 + (n - 1)(5)              |
| 187 - 2 = 5n - 5                  |
| 185 + 5 = 5n                      |
| 190/5 = n                         |
| n = 38                            |

> S<sub>n</sub> =
> $$ {n} \over {2} $$
> (a + t<sub>n</sub>)

We know that there are 38 terms in the series and that the 38th term is 187.

| Solution                              |
| :------------------------------------ |
| S<sub>38</sub> = 38/2(2 + 187) = 3591 |

<br>

# Exponential Growth and Geometric Sequences

An electric heater is now worth $100. Its value increases by 9% every year. How much will the heater be worth after 8 years?

| Year | Value ($) | Method                 | Analysis               |
| :--- | :-------- | :--------------------- | :--------------------- |
| 0    | 100.00    | 100                    | 100                    |
| 1    | 109.00    | 100 + 0.09 x 100.00    | 100 x 1.09<sup>1</sup> |
| 2    | 118.81    | 109.00 + 0.09 x 109.00 | 100 x 1.09<sup>2</sup> |

Noticing the pattern in the growth of the value, the value of the heater after 8 years is: 100(1.09)<sup>8</sup> = $199.26

This multiplicative growth is called exponential growth.

<br>

## 2. Geometric Sequence

In a geometric sequence, the quotient obtained by dividing any two consecutive terms is a constant. This constant "r is called the common ratio," where r =
$$ {{t}_{n+1}} \over {t_n} $$

Ex) 1, 3, 9, 27, ... &rarr; r = 3/1 = 3

## Example: 2. Geometric Sequence

State r of geometric sequence: 3, -12, 48, -192, ...

> r =
> $$ {{t}_{n+1}} \over {t_n} $$

| Solution       |
| :------------- |
| r = -12/3 = -4 |

<br>

## 2 - a. General term of the geometric sequence

a, ar, ar<sup>2</sup>, ar<sup>3</sup>, ... is t<sub>n</sub> = a r<sup>n-1</sup>

Ex) Determine the 11th term of the geometric sequence "3, 6, 12, 24, ..."

a = 3 and r = 6/3 = 2, n - 1 = 11 - 1 = 10

| Solution                                  |
| :---------------------------------------- |
| t<sub>11</sub> = 3(2)<sup>10</sup> = 3072 |

## Example: 2 - a. General term of the geometric sequence

Write the general term for the geometric sequence: 1, -2, 4, -8, ...

> t<sub>n</sub> = a r<sup>n-1</sup>

a = 1, r = -2/1 = -2

t<sub>n</sub> = 1 (-2)<sup>n-1</sup> = (-2)<sup>n-1</sup>

<br>

## 2 - b. The Sum of a Geometric Series

For the general geometric series "a + ar + ar<sup>2</sup> + ar<sup>3</sup> + ...," the sum of the first n terms is S<sub>n</sub> =
$$ {a(r^n - 1)} \over {r - 1} $$
, where r ‚â† 1.

Ex) Determine the sum of the first 8 terms of the geometric series: "6 + 24 + 96 + ..."

a = 6, r = 24/6 = 4, n = 8

> S<sub>n</sub> =
> $$ {a(r^n - 1)} \over {r - 1} $$

| Solution                                               |
| :----------------------------------------------------- |
| S<sub>8</sub> = 6(4<sup>8</sup> - 1)/(4 - 1) = 131,070 |

## Example: 2 - b. The Sum of a Geometric Series

Determine the sum of the first 12 terms of the geometric series: "1 ‚Äì 2 + 4 ‚Äì 8 + ..."

> S<sub>n</sub> =
> $$ {a(r^n - 1)} \over {r - 1} $$

a = 1, r = -2, n = 12

S<sub>12</sub> =
$$ {1((-2)^(12) - 1)} \over {-2 - 1} $$
= 
$$ {(4096 - 1)} \over {-3} $$
=
$$ {4095} \over {-3} $$
= -1365

<br>

# Exercise

## eCentennial/Content/Course Documents/Math175 Supplement: Page 17 and 18 All!

<br>

---

<br>

    üñãÔ∏è This is my self-taught blog! Feel free to let me know
    if there are some errors or wrong parts üòÜ

[Back to Top](#){: .btn .btn--primary }{: .align-right}
